src/Sound/Semantics/Omni.dfy
@@ -106,21 +106,12 @@ module Omni {
       && v.IsDefinedOn(|st|) 
       && st[x := st.Eval(v)] in post
     case Call(proc, args) =>
-      // var Pre := SeqSubstitute(proc.Pre, args.ToExpr());
-      // var Post := SeqSubstitute(proc.Post, args.ToExpr());
-      // var outVars := args.OutArgs();
-      // && (forall v <- outVars :: v < |st|)
-      // && (forall e <- Pre :: e.IsDefinedOn(|st|) && st.Eval(e))
-      // && forall st': State :: (
-      //   && st' in st.EqExcept(outVars)
-      //   && (forall e <- Post :: e.IsDefinedOn(|st'|) && st'.Eval(e)))
-      //     ==> st' in post
       && args.IsDefinedOn(|st|)
       && var callSt := args.EvalOn(st);
         && (forall e <- proc.Pre :: e.IsDefinedOn(|callSt|) && callSt.Eval(e))
         && forall st': State :: (
           && st' in st.EqExcept(args.OutArgs())
-          && var callSt' := args.EvalOn(st');
+          && var callSt' := args.EvalOn(st') + args.EvalOldOn(st);
             (forall e <- proc.Post :: e.IsDefinedOn(|callSt'|) && callSt'.Eval(e)))
               ==> st' in post
   }
